src/phase2/flexible_completion.lean
@@ -1,0 +1,49 @@
+import phase2.approximation
+
+open set
+open_locale cardinal classical
+
+universe u
+
+namespace con_nf
+variables [params.{u}] {α : Λ} [core_tangle_cumul α] [positioned_tangle_cumul α]
+  [position_data.{}] [almost_tangle_cumul α]
+
+namespace near_litter_approx
+
+variables (α) {β : type_index} (π : near_litter_approx) (A : extended_index β)
+
+def id_on_flexible : local_perm litter := {
+  to_fun := id,
+  inv_fun := id,
+  domain := {L | flexible α L A} \ π.litter_perm.domain,
+  to_fun_domain' := λ L h, h,
+  inv_fun_domain' := λ L h, h,
+  left_inv' := λ L h, rfl,
+  right_inv' := λ L h, rfl,
+}
+
+lemma id_on_flexible_domain :
+  (id_on_flexible α π A).domain = {L | flexible α L A} \ π.litter_perm.domain := rfl
+
+lemma id_on_flexible_domain_disjoint :
+  disjoint π.litter_perm.domain (id_on_flexible α π A).domain :=
+by rw [disjoint_iff_inter_eq_empty, id_on_flexible_domain, inter_diff_self]
+
+noncomputable def flexible_completion_litter_perm : local_perm litter :=
+local_perm.piecewise π.litter_perm (id_on_flexible α π A) (id_on_flexible_domain_disjoint α π A)
+
+lemma flexible_completion_litter_perm_domain :
+  (flexible_completion_litter_perm α π A).domain = π.litter_perm.domain ∪ {L | flexible α L A} :=
+by rw [flexible_completion_litter_perm, local_perm.piecewise_domain,
+  id_on_flexible_domain, union_diff_self]
+
+noncomputable def flexible_completion : near_litter_approx := {
+  atom_perm := π.atom_perm,
+  litter_perm := flexible_completion_litter_perm α π A,
+  domain_small := π.domain_small,
+}
+
+end near_litter_approx
+
+end con_nf
